Add transaction info to external calls
Progress on #5

vyperTestScript.sml
@@ -42,11 +42,32 @@ val () = cv_trans_deep_embedding EVAL test_if_control_flow_ast_def;
 
 val pair_case_rand = TypeBase.case_rand_of``:'a # 'b``
 
+val contract_addr = “42w: address”
+val sender_addr = “1001w: address”
+
+Definition call_foo_tx_def:
+  call_foo_tx = transaction ^sender_addr ^contract_addr "foo" [] 0
+End
+
+Definition call_bar_tx_def:
+  call_bar_tx = transaction ^sender_addr ^contract_addr "bar" [] 0
+End
+
+Theorem call_foo_tx_target[simp]:
+  call_foo_tx.target = 42w ∧
+  call_bar_tx.target = 42w
+Proof
+  rw[call_foo_tx_def, call_bar_tx_def]
+QED
+
+val () = cv_trans_deep_embedding EVAL call_foo_tx_def;
+val () = cv_trans_deep_embedding EVAL call_bar_tx_def;
+
 Theorem test_if_control_flow:
   FST $ external_call
     (load_contract initial_machine_state
-       addr test_if_control_flow_ast)
-    addr "foo" []
+       ^contract_addr test_if_control_flow_ast)
+    call_foo_tx
   = INL (IntV 44)
 Proof
   rw[external_call_def, load_contract_def, initial_machine_state_def,
@@ -73,8 +94,8 @@ val () = cv_trans_deep_embedding EVAL test_for_control_flow_ast_def;
 Theorem test_for_control_flow:
   FST $ external_call
     (load_contract initial_machine_state
-       addr test_for_control_flow_ast)
-    addr "foo" []
+       ^contract_addr test_for_control_flow_ast)
+    call_foo_tx
   = INL (IntV 6)
 Proof
   rw[external_call_def, load_contract_def, initial_machine_state_def,
@@ -102,8 +123,8 @@ val () = cv_trans_deep_embedding EVAL test_array_assign_ast_def;
 Theorem test_array_assign:
   FST $ external_call
    (load_contract initial_machine_state
-      addr test_array_assign_ast)
-    addr "foo" []
+      ^contract_addr test_array_assign_ast)
+    call_foo_tx
   = INL (IntV 47)
 Proof
   rw[external_call_def, load_contract_def, initial_machine_state_def,
@@ -131,8 +152,8 @@ val () = cv_trans_deep_embedding EVAL test_storage_array_assign_ast_def;
 Theorem test_storage_array_assign:
   FST $ external_call
    (load_contract initial_machine_state
-      addr test_storage_array_assign_ast)
-    addr "foo" []
+      ^contract_addr test_storage_array_assign_ast)
+    call_foo_tx
   = INL (IntV 5)
 Proof
   rw[external_call_def, load_contract_def, initial_machine_state_def,
@@ -168,8 +189,8 @@ val () = cv_trans_deep_embedding EVAL test_internal_call_ast_def;
 Theorem test_internal_call:
   FST $ external_call
    (load_contract initial_machine_state
-      addr test_internal_call_ast)
-    addr "foo" []
+      ^contract_addr test_internal_call_ast)
+    call_foo_tx
   = INL (IntV 12)
 Proof
   rw[external_call_def, load_contract_def, initial_machine_state_def,
@@ -195,8 +216,8 @@ val () = cv_trans_deep_embedding EVAL test_internal_call_without_return_ast_def;
 Theorem test_internal_call_without_return:
   FST $ external_call
    (load_contract initial_machine_state
-      addr test_internal_call_without_return_ast)
-    addr "foo" []
+      ^contract_addr test_internal_call_without_return_ast)
+    call_foo_tx
   = INL (IntV 42)
 Proof
   rw[external_call_def, load_contract_def, initial_machine_state_def,
@@ -224,8 +245,8 @@ val () = cv_trans_deep_embedding EVAL test_internal_call_with_args_ast_def;
 Theorem test_internal_call_with_args:
   FST $ external_call
    (load_contract initial_machine_state
-      addr test_internal_call_with_args_ast)
-    addr "foo" []
+      ^contract_addr test_internal_call_with_args_ast)
+    call_foo_tx
   = INL (IntV 6)
 Proof
   rw[external_call_def, load_contract_def, initial_machine_state_def,
@@ -253,8 +274,8 @@ val () = cv_trans_deep_embedding EVAL test_internal_call_with_args2_ast_def;
 Theorem test_internal_call_with_args2:
   FST $ external_call
    (load_contract initial_machine_state
-      addr test_internal_call_with_args2_ast)
-    addr "foo" []
+      ^contract_addr test_internal_call_with_args2_ast)
+    call_foo_tx
   = INL (IntV 6)
 Proof
   rw[external_call_def, load_contract_def, initial_machine_state_def,
@@ -281,8 +302,8 @@ val () = cv_trans_deep_embedding EVAL test_storage_variables_ast_def;
 Theorem test_storage_variables:
   FST $ external_call
    (load_contract initial_machine_state
-      addr test_storage_variables_ast)
-    addr "foo" []
+      ^contract_addr test_storage_variables_ast)
+    call_foo_tx
   = INL (IntV 43)
 Proof
   rw[external_call_def, load_contract_def, initial_machine_state_def,
@@ -308,8 +329,8 @@ val () = cv_trans_deep_embedding EVAL test_storage_variables2_ast_def;
 Theorem test_storage_variables2:
   FST $ external_call
    (load_contract initial_machine_state
-      addr test_storage_variables2_ast)
-    addr "foo" []
+      ^contract_addr test_storage_variables2_ast)
+    call_foo_tx
   = INL (IntV 3)
 Proof
   rw[external_call_def, load_contract_def, initial_machine_state_def,
@@ -345,8 +366,8 @@ val () = cv_trans_deep_embedding EVAL test_storage_variables3_ast_def;
 Theorem test_storage_variables3:
   FST $ external_call
    (load_contract initial_machine_state
-      addr test_storage_variables3_ast)
-    addr "foo" []
+      ^contract_addr test_storage_variables3_ast)
+    call_foo_tx
   = INL (IntV 12)
 Proof
   rw[external_call_def, load_contract_def, initial_machine_state_def,
@@ -367,13 +388,13 @@ End
 val () = cv_trans_deep_embedding EVAL test_statefulness_of_storage_ast_def;
 
 Theorem test_statefulness_of_storage:
-  let ms = load_contract initial_machine_state addr
+  let ms = load_contract initial_machine_state ^contract_addr
              test_statefulness_of_storage_ast in
-  let (r1, ms) = external_call ms addr "foo" [] in
-  let (r2, ms) = external_call ms addr "foo" [] in
-  let (r3, ms) = external_call ms addr "foo" [] in
-  let (r4, ms) = external_call ms addr "foo" [] in
-  let (r5, ms) = external_call ms addr "foo" [] in
+  let (r1, ms) = external_call ms call_foo_tx in
+  let (r2, ms) = external_call ms call_foo_tx in
+  let (r3, ms) = external_call ms call_foo_tx in
+  let (r4, ms) = external_call ms call_foo_tx in
+  let (r5, ms) = external_call ms call_foo_tx in
     r1 = INL (IntV 1) ∧
     r2 = INL (IntV 2) ∧
     r3 = INL (IntV 3) ∧
@@ -402,18 +423,18 @@ End
 val () = cv_trans_deep_embedding EVAL test_statefulness_of_storage2_ast_def;
 
 Theorem test_statefulness_of_storage2:
-  let ms = load_contract initial_machine_state addr
+  let ms = load_contract initial_machine_state ^contract_addr
              test_statefulness_of_storage2_ast in
-  let (f1, ms) = external_call ms addr "foo" [] in
-  let (b1, ms) = external_call ms addr "bar" [] in
-  let (f2, ms) = external_call ms addr "foo" [] in
-  let (b2, ms) = external_call ms addr "bar" [] in
-  let (f3, ms) = external_call ms addr "foo" [] in
-  let (b3, ms) = external_call ms addr "bar" [] in
-  let (f4, ms) = external_call ms addr "foo" [] in
-  let (b4, ms) = external_call ms addr "bar" [] in
-  let (f5, ms) = external_call ms addr "foo" [] in
-  let (b5, ms) = external_call ms addr "bar" [] in
+  let (f1, ms) = external_call ms call_foo_tx in
+  let (b1, ms) = external_call ms call_bar_tx in
+  let (f2, ms) = external_call ms call_foo_tx in
+  let (b2, ms) = external_call ms call_bar_tx in
+  let (f3, ms) = external_call ms call_foo_tx in
+  let (b3, ms) = external_call ms call_bar_tx in
+  let (f4, ms) = external_call ms call_foo_tx in
+  let (b4, ms) = external_call ms call_bar_tx in
+  let (f5, ms) = external_call ms call_foo_tx in
+  let (b5, ms) = external_call ms call_bar_tx in
     f1 = INL (IntV (0 * 2 + 1)) ∧
     f2 = INL (IntV (1 * 2 + 1)) ∧
     f3 = INL (IntV (2 * 2 + 1)) ∧
@@ -448,8 +469,8 @@ val () = cv_trans_deep_embedding EVAL test_tstorage_variables0_ast_def;
 Theorem test_tstorage_variables0:
   FST $ external_call
    (load_contract initial_machine_state
-      addr test_tstorage_variables0_ast)
-    addr "foo" []
+      ^contract_addr test_tstorage_variables0_ast)
+    call_foo_tx
   = INL (IntV 3)
 Proof
   rw[external_call_def, load_contract_def, initial_machine_state_def,
@@ -477,8 +498,8 @@ val () = cv_trans_deep_embedding EVAL test_tstorage_variables2_ast_def;
 Theorem test_tstorage_variables2:
   FST $ external_call
    (load_contract initial_machine_state
-      addr test_tstorage_variables2_ast)
-    addr "foo" []
+      ^contract_addr test_tstorage_variables2_ast)
+    call_foo_tx
   = INL (IntV 3)
 Proof
   rw[external_call_def, load_contract_def, initial_machine_state_def,
@@ -545,8 +566,8 @@ val () = cv_trans_deep_embedding EVAL test_default_storage_values_ast_def;
 Theorem test_default_storage_values:
   FST $ external_call
    (load_contract initial_machine_state
-      addr test_default_storage_values_ast)
-    addr "foo" []
+      ^contract_addr test_default_storage_values_ast)
+    call_foo_tx
   = INL (IntV 1)
 Proof
   rw[external_call_def, load_contract_def, initial_machine_state_def,
@@ -571,8 +592,8 @@ val () = cv_trans_deep_embedding EVAL test_len_builtin_ast_def;
 Theorem test_len_builtin:
   FST $ external_call
    (load_contract initial_machine_state
-      addr test_len_builtin_ast)
-    addr "foo" []
+      ^contract_addr test_len_builtin_ast)
+    call_foo_tx
   = INL (IntV 3)
 Proof
   rw[external_call_def, load_contract_def, initial_machine_state_def,
@@ -594,8 +615,8 @@ val () = cv_trans_deep_embedding EVAL test_len_builtin2_ast_def;
 Theorem test_len_builtin2:
   FST $ external_call
    (load_contract initial_machine_state
-      addr test_len_builtin2_ast)
-    addr "foo" []
+      ^contract_addr test_len_builtin2_ast)
+    call_foo_tx
   = INL (IntV 0)
 Proof
   rw[external_call_def, load_contract_def, initial_machine_state_def,
@@ -618,8 +639,8 @@ val () = cv_trans_deep_embedding EVAL test_len_builtin3_ast_def;
 Theorem test_len_builtin3:
   FST $ external_call
    (load_contract initial_machine_state
-      addr test_len_builtin3_ast)
-    addr "foo" []
+      ^contract_addr test_len_builtin3_ast)
+    call_foo_tx
   = INL (IntV 5)
 Proof
   rw[external_call_def, load_contract_def, initial_machine_state_def,
@@ -644,8 +665,8 @@ val () = cv_trans_deep_embedding EVAL test_len_builtin4_ast_def;
 Theorem test_len_builtin4:
   FST $ external_call
    (load_contract initial_machine_state
-      addr test_len_builtin4_ast)
-    addr "foo" []
+      ^contract_addr test_len_builtin4_ast)
+    call_foo_tx
   = INL (IntV 5)
 Proof
   rw[external_call_def, load_contract_def, initial_machine_state_def,
@@ -672,8 +693,8 @@ val () = cv_trans_deep_embedding EVAL test_external_func_arg_ast_def;
 Theorem test_external_func_arg:
   FST $ external_call
    (load_contract initial_machine_state
-      addr test_external_func_arg_ast)
-    addr "foo" [IntV 42]
+      ^contract_addr test_external_func_arg_ast)
+    (transaction ^sender_addr ^contract_addr "foo" [IntV 42] 0)
   = INL (IntV 42)
 Proof
   rw[external_call_def, load_contract_def, initial_machine_state_def,
